code/ecdsap256sha2/Hacl.Impl.LowLevel.fst
@@ -826,3 +826,26 @@ let copy_conditional out x mask =
 
   lemma_eq_funct_ (as_seq h1 out) (as_seq h0 out);
   lemma_eq_funct_ (as_seq h1 out) (as_seq h0 x)
+
+
+
+val toUint64: i: lbuffer uint8 (32ul) -> o: felem -> Stack unit
+  (requires fun h -> live h i /\ live h o /\ disjoint i o)
+  (ensures fun h0 _ h1 -> 
+    modifies (loc o) h0 h1 /\ 
+    as_seq h1 o == Lib.ByteSequence.uints_from_bytes_le (as_seq h0 i)
+  )
+
+let toUint64 i o = 
+  Lib.ByteBuffer.uints_from_bytes_le o i
+
+
+val toUint8: i: felem ->  o: lbuffer uint8 (32ul) -> Stack unit
+  (requires fun h -> live h i /\ live h o /\ disjoint i o)
+  (ensures fun h0 _ h1 -> 
+    modifies (loc o) h0 h1 /\ 
+    as_seq h1 o == Lib.ByteSequence.uints_to_bytes_le #_ #_ #4 (as_seq h0 i)
+  )
+
+let toUint8 i o = 
+  Lib.ByteBuffer.uints_to_bytes_le (size 4) o i
